feat(IntProp): Kripke Completeness for `𝐊𝐂` and `𝐋𝐂` (#118)
* wip

* LC completed

* done

* fx

Logic/Logic/HilbertStyle/Supplemental.lean
@@ -13,6 +13,13 @@ open NegationEquiv
 open FiniteContext
 open List
 
+def mdp_in : 𝓢 ⊢ p ⋏ (p ⟶ q) ⟶ q := by
+  apply deduct';
+  have hp  : [p, p ⟶ q] ⊢[𝓢] p := FiniteContext.byAxm;
+  have hpq : [p, p ⟶ q] ⊢[𝓢] p ⟶ q := FiniteContext.byAxm;
+  exact hpq ⨀ hp;
+lemma mdp_in! : 𝓢 ⊢! p ⋏ (p ⟶ q) ⟶ q := ⟨mdp_in⟩
+
 def bot_of_mem_either [System.NegationEquiv 𝓢] (h₁ : p ∈ Γ) (h₂ : ~p ∈ Γ) : Γ ⊢[𝓢] ⊥ := by
   have hp : Γ ⊢[𝓢] p := FiniteContext.byAxm h₁;
   have hnp : Γ ⊢[𝓢] p ⟶ ⊥ := neg_equiv'.mp $ FiniteContext.byAxm h₂;
@@ -614,6 +621,11 @@ lemma iff_concat_conj! : 𝓢 ⊢! ⋀(Γ ++ Δ) ⟷ ⋀Γ ⋏ ⋀Δ := by
   apply iff_intro!;
   . apply deduct'!; apply iff_concat_conj'!.mp; exact id!;
   . apply deduct'!; apply iff_concat_conj'!.mpr; exact id!;
+
+lemma imply_left_conj_concat! : 𝓢 ⊢! ⋀(Γ ++ Δ) ⟶ p ↔ 𝓢 ⊢! (⋀Γ ⋏ ⋀Δ) ⟶ p := by
+  constructor;
+  . intro h; exact imp_trans''! (and₂'! iff_concat_conj!) h;
+  . intro h; exact imp_trans''! (and₁'! iff_concat_conj!) h;
 
 end Conjunction
 
