Logic/Propositional/Superintuitionistic/Kripke/Completeness.lean
@@ -328,7 +328,7 @@ lemma lindenbaum (hCon : (Λ)-Consistent t₀) : ∃ (t : SaturatedConsistentTab
 
 instance [System.Consistent Λ] : Nonempty (SCT Λ) := ⟨lindenbaum Tableau.self_ParametricConsistent |>.choose⟩
 
-variable (t : SCT Λ)
+variable {t : SCT Λ}
 
 @[simp] lemma disjoint : Disjoint t.tableau.1 t.tableau.2 := t.tableau.disjoint_of_consistent t.consistent
 
@@ -351,12 +351,15 @@ lemma equality_of₂ (e₂ : t₁.tableau.2 = t₂.tableau.2) : t₁ = t₂ := e
 
 lemma not_mem₂ {Γ : List (Formula α)} (hΓ : ∀ p ∈ Γ, p ∈ t.tableau.1) (h : Λ ⊢! ⋀Γ ⟶ q) : q ∉ t.tableau.2 := t.tableau.not_mem₂ t.consistent hΓ h
 
-lemma mdp₁ (hp : p ∈ t.tableau.1) (h : Λ ⊢! p ⟶ q) : q ∈ t.tableau.1 := by
-  exact t.not_mem₂_iff_mem₁.mp $ not_mem₂ (by simpa) (show Λ ⊢! ⋀[p] ⟶ q by simpa;)
+lemma mdp₁ (hp₁ : p ∈ t.tableau.1) (h : Λ ⊢! p ⟶ q) : q ∈ t.tableau.1 := by
+  apply not_mem₂_iff_mem₁.mp;
+  by_contra hq₂;
+  have : Λ ⊬! p ⟶ q := by simpa using t.consistent (Γ := [p]) (Δ := [q]) (by simpa) (by simpa);
+  contradiction;
 
 @[simp]
 lemma mem₁_verum : ⊤ ∈ t.tableau.1 := by
-  apply t.not_mem₂_iff_mem₁.mp;
+  apply not_mem₂_iff_mem₁.mp;
   by_contra hC;
   have : Λ ⊬! ⋀[] ⟶ ⋁[⊤] := t.consistent (by simp) (by simpa);
   have : Λ ⊢! ⋀[] ⟶ ⋁[⊤] := by simp;
@@ -374,18 +377,33 @@ lemma iff_mem₁_and : p ⋏ q ∈ t.tableau.1 ↔ p ∈ t.tableau.1 ∧ q ∈ t
   constructor;
   . intro h; constructor <;> exact mdp₁ h (by simp)
   . rintro ⟨hp, hq⟩;
+    apply not_mem₂_iff_mem₁.mp;
     by_contra hC;
     have : Λ ⊢! ⋀[p, q] ⟶ ⋁[p ⋏ q] := by simp;
-    have : Λ ⊬! ⋀[p, q] ⟶ ⋁[p ⋏ q] := t.consistent (by aesop) (by simpa using t.not_mem₁_iff_mem₂.mp hC);
+    have : Λ ⊬! ⋀[p, q] ⟶ ⋁[p ⋏ q] := t.consistent (by simp_all) (by simp_all);
     contradiction;
+
+lemma iff_mem₁_conj {Γ : List (Formula α)} : ⋀Γ ∈ t.tableau.1 ↔ ∀ p ∈ Γ, p ∈ t.tableau.1 := by
+  induction Γ using List.induction_with_singleton with
+  | hnil => simp;
+  | hsingle p => simp;
+  | hcons p Γ Γ_nil ih =>
+    simp only [(List.conj₂_cons_nonempty Γ_nil), List.mem_cons];
+    constructor;
+    . rintro h p (rfl | hp);
+      . exact iff_mem₁_and.mp h |>.1;
+      . exact ih.mp (iff_mem₁_and.mp h |>.2) _ hp;
+    . intro h;
+      apply iff_mem₁_and.mpr;
+      simp_all;
 
 @[simp]
 lemma iff_mem₁_or : p ⋎ q ∈ t.tableau.1 ↔ p ∈ t.tableau.1 ∨ q ∈ t.tableau.1 := by
   constructor;
   . intro h;
-    by_contra hC; simp [not_or] at hC;
-    have : p ∈ t.tableau.2 := t.not_mem₁_iff_mem₂.mp hC.1;
-    have : q ∈ t.tableau.2 := t.not_mem₁_iff_mem₂.mp hC.2;
+    by_contra hC; push_neg at hC;
+    have : p ∈ t.tableau.2 := not_mem₁_iff_mem₂.mp hC.1;
+    have : q ∈ t.tableau.2 := not_mem₁_iff_mem₂.mp hC.2;
     have : Λ ⊢! ⋀[p ⋎ q] ⟶ ⋁[p, q] := by simp;
     have : Λ ⊬! ⋀[p ⋎ q] ⟶ ⋁[p, q] := t.consistent (by simp_all) (by simp_all);
     contradiction;
@@ -394,9 +412,28 @@ lemma iff_mem₁_or : p ⋎ q ∈ t.tableau.1 ↔ p ∈ t.tableau.1 ∨ q ∈ t.
     | inl h => exact mdp₁ h or₁!
     | inr h => exact mdp₁ h or₂!
 
+lemma not_mem₁_neg_of_mem₁ : p ∈ t.tableau.1 → ~p ∉ t.tableau.1 := by
+  intro hp;
+  by_contra hnp;
+  have := iff_mem₁_and.mpr ⟨hp, hnp⟩;
+  have : ⊥ ∈ t.tableau.1 := mdp₁ (q := ⊥) this (by simp);
+  have : ⊥ ∉ t.tableau.1 := not_mem₁_falsum
+  contradiction;
+
+lemma mem₂_neg_of_mem₁ : p ∈ t.tableau.1 → ~p ∈ t.tableau.2 := by
+  intro h;
+  exact not_mem₁_iff_mem₂ (p := ~p) (t := t) |>.mp $ not_mem₁_neg_of_mem₁ h;
+
 lemma mem₁_of_provable : Λ ⊢! p → p ∈ t.tableau.1 := by
   intro h;
   exact mdp₁ mem₁_verum $ dhyp! h;
+
+lemma mdp₁_mem (hp : p ∈ t.tableau.1) (h : p ⟶ q ∈ t.tableau.1) : q ∈ t.tableau.1 := by
+  apply not_mem₂_iff_mem₁.mp;
+  by_contra hC;
+  have : Λ ⊬! (p ⋏ (p ⟶ q)) ⟶ q := t.consistent (Γ := [p, p ⟶ q]) (Δ := [q]) (by aesop) (by simpa);
+  have : Λ ⊢! (p ⋏ (p ⟶ q)) ⟶ q := mdp_in!
+  contradiction;
 
 end SaturatedConsistentTableau
 
@@ -427,6 +464,115 @@ lemma transitive : Transitive (CanonicalFrame Λ) := by
   simp [CanonicalFrame];
   intro x y z;
   apply Set.Subset.trans;
+
+open Classical in
+lemma confluent [HasAxiomWeakLEM Λ] : Confluent (CanonicalFrame Λ) := by
+  simp [Confluent, CanonicalFrame];
+  intro x y z Rxy Rxz;
+  suffices (Λ)-Consistent (y.tableau.1 ∪ z.tableau.1, ∅) by
+    obtain ⟨w, hw⟩ := lindenbaum (Λ := Λ) this;
+    use w;
+    simp_all;
+
+  intro Γ Δ;
+  intro hΓ hΔ h;
+  simp_all;
+  have := List.nil_iff.mpr hΔ; subst this; simp at h; clear hΔ;
+
+  have hΓy : ¬(∀ w, w ∈ Γ → w ∈ y.tableau.1) := by
+    by_contra hC;
+    have := by simpa using y.consistent (Γ := Γ) (Δ := []) hC (by simp);
+    contradiction;
+  push_neg at hΓy;
+
+  have hΓz : ¬(∀ w, w ∈ Γ → w ∈ z.tableau.1) := by
+    by_contra hC;
+    have := by simpa using z.consistent (Γ := Γ) (Δ := []) hC (by simp);
+    contradiction;
+  push_neg at hΓz;
+
+  let Θy := Γ.filter (λ p => p ∈ y.tableau.1 ∧ p ∉ x.tableau.1);
+  let Θz := Γ.filter (λ p => p ∈ z.tableau.1 ∧ p ∉ x.tableau.1);
+  let Θx := Γ.filter (λ p => (p ∈ y.tableau.1 ∧ p ∈ x.tableau.1) ∨ (p ∈ z.tableau.1 ∧ p ∈ x.tableau.1));
+
+  suffices ~⋀Θy ∈ x.tableau.1 by
+    have : ~⋀Θy ∈ y.tableau.1 := Rxy this;
+    have : ⋀Θy ∈ y.tableau.1 := iff_mem₁_conj.mpr $ by
+      intro p hp;
+      have := by simpa using List.of_mem_filter hp;
+      exact this.1;
+    have : Λ ⊬! ⋀Θy ⋏ ~⋀Θy ⟶ ⊥ := y.consistent (Γ := [⋀Θy, ~⋀Θy]) (Δ := []) (by simp; constructor <;> assumption) (by simp);
+    have : Λ ⊢! ⋀Θy ⋏ ~⋀Θy ⟶ ⊥ := by simp;
+    contradiction;
+
+  have : Λ ⊢! (⋀Θx ⋏ (⋀Θy ⋏ ⋀Θz)) ⟶ ⊥ := imp_trans''! (by
+    -- TODO: need more refactor
+    have d₁ : Λ ⊢! ⋀Θx ⋏ ⋀(Θy ++ Θz) ⟶ ⋀(Θx ++ (Θy ++ Θz)) := and₂'! $ iff_concat_conj!;
+    have d₂ : Λ ⊢! ⋀Θy ⋏ ⋀Θz ⟶ ⋀(Θy ++ Θz) := and₂'! $ iff_concat_conj!;
+    have d₃ : Λ ⊢! ⋀Θx ⋏ ⋀Θy ⋏ ⋀Θz ⟶ ⋀(Θx ++ (Θy ++ Θz)) := imp_trans''! (by
+      apply deduct'!;
+      have : [⋀Θx ⋏ ⋀Θy ⋏ ⋀Θz] ⊢[Λ]! ⋀Θx ⋏ ⋀Θy ⋏ ⋀Θz := FiniteContext.by_axm!;
+      apply and₃'!;
+      . exact and₁'! this;
+      . exact (FiniteContext.of'! d₂) ⨀ (and₂'! this);
+    ) d₁;
+    exact imp_trans''! d₃ $ conjconj_subset! $ by
+      intro p hp; simp;
+      apply or_iff_not_imp_left.mpr;
+      intro nmem_Θx;
+      have := (not_imp_not.mpr $ List.mem_filter_of_mem hp) nmem_Θx; simp at this;
+      have ⟨hy₁, hz₁⟩ := this;
+      rcases hΓ _ hp with (hy | hz);
+      . left;
+        apply List.mem_filter_of_mem hp;
+        simp;
+        constructor;
+        . assumption;
+        . exact hy₁ hy;
+      . right;
+        apply List.mem_filter_of_mem hp;
+        simp;
+        constructor;
+        . assumption;
+        . exact hz₁ hz;
+  ) h;
+  have : Λ ⊢! ⋀Θx ⟶ ⋀Θy ⟶ ~⋀Θz := and_imply_iff_imply_imply'!.mp $
+    (imp_trans''! (and_imply_iff_imply_imply'!.mp $ imp_trans''! (and₁'! and_assoc!) this) (and₂'! $ neg_equiv!));
+  have d : Λ ⊢! ⋀Θx ⟶ ~~⋀Θz ⟶ ~⋀Θy := imp_trans''! this contra₀!;
+
+  have mem_Θx_x : ⋀Θx ∈ x.tableau.1 := iff_mem₁_conj.mpr $ by
+    intro p hp;
+    have := by simpa using List.of_mem_filter hp;
+    rcases this with ⟨_, _⟩ | ⟨_, _⟩ <;> assumption;
+  have mem_Θz_z : ⋀Θz ∈ z.tableau.1 := iff_mem₁_conj.mpr $ by
+    intro p hp;
+    have := by simpa using List.of_mem_filter hp;
+    exact this.1;
+
+  have nmem_nΘz_z : ~⋀Θz ∉ z.tableau.1 := not_mem₁_neg_of_mem₁ mem_Θz_z;
+  have nmem_nΘz_x : ~⋀Θz ∉ x.tableau.1 := Set.not_mem_subset Rxz nmem_nΘz_z;
+  have mem_nnΘz_x : ~~⋀Θz ∈ x.tableau.1 := or_iff_not_imp_left.mp (iff_mem₁_or.mp $ mem₁_of_provable $ wlem!) nmem_nΘz_x;
+
+  exact mdp₁_mem mem_nnΘz_x $ mdp₁ mem_Θx_x d;
+
+
+lemma connected [HasAxiomDummett Λ] : Connected (CanonicalFrame Λ) := by
+  simp [Connected, CanonicalFrame];
+  intro x y z Rxy Ryz;
+  apply or_iff_not_imp_left.mpr;
+  intro nRyz;
+  obtain ⟨p, hyp, nhzp⟩ := Set.not_subset.mp nRyz;
+  intro q hqz;
+  have : q ⟶ p ∉ x.tableau.1 := by
+    by_contra hqpx;
+    have hqpz : q ⟶ p ∈ z.tableau.1 := by aesop;
+    have : p ∈ z.tableau.1 := mdp₁_mem hqz hqpz;
+    contradiction;
+  have := iff_mem₁_or.mp $ mem₁_of_provable (t := x) (p := (p ⟶ q) ⋎ (q ⟶ p)) dummett!;
+  have hpqx : p ⟶ q ∈ x.tableau.1 := by aesop;
+  have hpqy : p ⟶ q ∈ y.tableau.1 := Rxy hpqx;
+  have : q ∈ y.tableau.1 := mdp₁_mem hyp hpqy;
+  exact this;
 
 end CanonicalFrame
 
@@ -467,7 +613,7 @@ private lemma truthlemma.himp
   . contrapose;
     simp_all [Satisfies];
     intro h;
-    replace h := t.not_mem₁_iff_mem₂.mp h;
+    replace h := not_mem₁_iff_mem₂.mp h;
     obtain ⟨t', ⟨h, _⟩⟩ := lindenbaum (Λ := Λ) (t₀ := (insert p t.tableau.1, {q})) $ by
       simp only [Tableau.ParametricConsistent];
       intro Γ Δ hΓ hΔ;
@@ -492,14 +638,14 @@ private lemma truthlemma.himp
     . simp_all only [Set.singleton_subset_iff];
     . constructor;
       . assumption;
-      . apply t'.not_mem₁_iff_mem₂.mpr;
+      . apply not_mem₁_iff_mem₂.mpr;
         simp_all only [Set.singleton_subset_iff];
   . simp [Satisfies.imp_def];
     intro h t' htt' hp;
     replace hp := ihp.mp hp;
     have hpq := htt' h;
     apply ihq.mpr;
-    apply t'.not_mem₂_iff_mem₁.mp;
+    apply not_mem₂_iff_mem₁.mp;
     exact not_mem₂
       (by simp_all)
       (show Λ ⊢! ⋀[p, p ⟶ q] ⟶ q by
@@ -518,7 +664,7 @@ private lemma truthlemma.hneg
   . contrapose;
     simp_all [Satisfies];
     intro h;
-    replace h := t.not_mem₁_iff_mem₂.mp h;
+    replace h := not_mem₁_iff_mem₂.mp h;
     obtain ⟨t', ⟨h, _⟩⟩ := lindenbaum (Λ := Λ) (t₀ := (insert p t.tableau.1, ∅)) $ by
       simp only [Tableau.ParametricConsistent];
       intro Γ Δ hΓ hΔ;
@@ -564,7 +710,7 @@ lemma deducible_of_validOnCanonicelModel : (CanonicalModel Λ) ⊧ p ↔ Λ ⊢!
     simp [ValidOnModel.iff_models, ValidOnModel]
     existsi t';
     apply truthlemma.not.mpr;
-    apply t'.not_mem₁_iff_mem₂.mpr;
+    apply not_mem₁_iff_mem₂.mpr;
     simp_all;
   . intro h t;
     suffices p ∈ t.tableau.1 by exact truthlemma.mpr this;
@@ -586,7 +732,7 @@ lemma complete (H : CanonicalFrame Λ ∈ 𝔽) {p : Formula α} : 𝔽#α ⊧ p
 
 instance instComplete (H : CanonicalFrame Λ ∈ 𝔽) : Complete Λ (𝔽#α) := ⟨complete H⟩
 
-instance Int_Complete : Complete (𝐈𝐧𝐭 : DeductionParameter α) (Kripke.ReflexiveTransitiveFrameClass.{u}#α) := instComplete $ by
+instance Int_complete : Complete 𝐈𝐧𝐭 (Kripke.ReflexiveTransitiveFrameClass.{u}#α) := instComplete $ by
   constructor;
   . exact CanonicalFrame.reflexive;
   . exact CanonicalFrame.transitive;
@@ -598,6 +744,21 @@ instance : Complete (𝐈𝐧𝐭 : DeductionParameter α) (Kripke.FrameClassOfS
   apply h;
   exact Kripke.Int_Characteraizable.characterize hF;
 ⟩
+
+
+instance LC_complete : Complete 𝐋𝐂 (Kripke.ReflexiveTransitiveConnectedFrameClass.{u}#α) := instComplete $ by
+  refine ⟨
+    CanonicalFrame.reflexive,
+    CanonicalFrame.transitive,
+    CanonicalFrame.connected
+  ⟩;
+
+instance KC_complete : Complete 𝐊𝐂 (Kripke.ReflexiveTransitiveConfluentFrameClass.{u}#α) := instComplete $ by
+  refine ⟨
+    CanonicalFrame.reflexive,
+    CanonicalFrame.transitive,
+    CanonicalFrame.confluent
+  ⟩;
 
 end
 
