Logic/Modal/Standard/Kripke/ModalCompanion.lean
@@ -101,7 +101,7 @@ open Formula
 lemma provable_S4_of_provable_efq : (𝐒𝟒 ⊢! pᵍ) → (𝐈𝐧𝐭 ⊢! p) := by
   contrapose;
   intro h;
-  replace h := (not_imp_not.mpr $ Superintuitionistic.Kripke.Int_Complete.complete) h;
+  replace h := (not_imp_not.mpr $ Superintuitionistic.Kripke.Int_complete.complete) h;
   simp [Semantics.Realize, ValidOnFrame, ValidOnModel] at h;
   obtain ⟨IF, ⟨IF_refl, IF_trans⟩, IV, IV_hered, w, hp⟩ := h;
 
