Logic/Propositional/Superintuitionistic/Kripke/DP.lean
@@ -116,8 +116,8 @@ theorem disjunctive_int : 𝐈𝐧𝐭 ⊢! p ⋎ q → 𝐈𝐧𝐭 ⊢! p ∨ 
   contrapose;
   intro hC; push_neg at hC;
   have ⟨hnp, hnq⟩ := hC;
-  obtain ⟨Fp, ⟨Fp_refl, Fp_trans⟩, Vp, Vp_hered, wp, hp⟩ := by simpa [Semantics.Realize, ValidOnFrame, ValidOnModel] using not_imp_not.mpr (@Kripke.Int_Complete α _ _ |>.complete) hnp;
-  obtain ⟨Fq, ⟨Fq_refl, Fq_trans⟩, Vq, Vq_hered, wq, hq⟩ := by simpa [Semantics.Realize, ValidOnFrame, ValidOnModel] using not_imp_not.mpr (@Kripke.Int_Complete α _ _ |>.complete) hnq;
+  obtain ⟨Fp, ⟨Fp_refl, Fp_trans⟩, Vp, Vp_hered, wp, hp⟩ := by simpa [Semantics.Realize, ValidOnFrame, ValidOnModel] using not_imp_not.mpr Int_complete.complete hnp;
+  obtain ⟨Fq, ⟨Fq_refl, Fq_trans⟩, Vq, Vq_hered, wq, hq⟩ := by simpa [Semantics.Realize, ValidOnFrame, ValidOnModel] using not_imp_not.mpr Int_complete.complete hnq;
   apply (not_imp_not.mpr Int_sound.sound);
   simp [Semantics.Realize, ValidOnFrame, ValidOnModel, Satisfies];
   use (IntDPCounterexampleFrame Fp Fq wp wq);
